formic_site_duct/converted_duct/obj/Debug/net6.0/formic_duct.AssemblyInfo.cs
@@ -13,7 +13,7 @@ using System.Reflection;
 [assembly: System.Reflection.AssemblyCompanyAttribute("formic_duct")]
 [assembly: System.Reflection.AssemblyConfigurationAttribute("Debug")]
 [assembly: System.Reflection.AssemblyFileVersionAttribute("1.0.0.0")]
-[assembly: System.Reflection.AssemblyInformationalVersionAttribute("1.0.0+c9ff703c3ff34200d85c88702c1d6a43f28db41c")]
+[assembly: System.Reflection.AssemblyInformationalVersionAttribute("1.0.0+7bbeee1f516b1cb20c1a978b32f38ab87d03129d")]
 [assembly: System.Reflection.AssemblyProductAttribute("formic_duct")]
 [assembly: System.Reflection.AssemblyTitleAttribute("formic_duct")]
 [assembly: System.Reflection.AssemblyVersionAttribute("1.0.0.0")]
