formic_site_duct/formic.apis.duct.dfy
@@ -18,19 +18,20 @@ module DuctApis {
             var catalog := new AllApiEndpoints();
 
             var formic_landing := new FormicLandingPage();
-            var home := new ApiEndpoint("/", ReturnType.Content(""), formic_landing);
+            var home := new ApiEndpoint("/", formic_landing);
             catalog.Add(home);
 
             var login_page := new LoginChallengePage();
-            var login := new ApiEndpoint("/login", ReturnType.ChallengeGoogle("/save_user"), login_page);
+            // The URL here is no longer used by the host, so we can simplify it.
+            var login := new ApiEndpoint("/login", login_page);
             catalog.Add(login);
 
             var save_user_page := new SaveUserPage();
-            var save_user := new ApiEndpoint("/save_user", ReturnType.Content(""), save_user_page);
+            var save_user := new ApiEndpoint("/save_user", save_user_page);
             catalog.Add(save_user);
 
             var secure_page := new SecurePage();
-            var secure := new ApiEndpoint("/secure", ReturnType.Content(""), secure_page);
+            var secure := new ApiEndpoint("/secure", secure_page);
             catalog.Add(secure);
             
             all := catalog; 
